cleaner version of ntt_rec3

crypto_examples/ntt_rec3.dfy
@@ -12,76 +12,106 @@ module ntt_recs3 {
     import opened ntt_recs2
     import opened ntt_rec
 
-   function method ntt_rec3_base(ghost a: seq<seq<elem>>, len: pow2_t, ghost idxs: seq<seq<index_t>>): (ys: seq<seq<elem>>)
-        requires ntt_chunk_indicies_inv(a, idxs, len);
-        requires len.full == 1 && len.exp == 0;
-        ensures ntt_chunks_eval_inv(a, idxs, ys, len);
+    function method chunk_count(m: pow2_t): nat
+        requires 0 <= m.exp <= L;
     {
-        nth_root_lemma();
-        var ys := seq(N, i requires 0 <= i < N => [Ar()[i]]);
-        assert ntt_chunks_eval_inv(a, idxs, ys, len) by {
-            forall ki: nat | ki < |a| 
-                ensures poly_eval_all_points(a[ki], ys[ki], len)
-            {
-                ntt_indicies_inv_consequence0(a[ki], idxs[ki], len, ki);
-                ntt_rec_base_case(a[ki], len);
-            }
-        }
-        ys
+        pow2_div(pow2(L), m).full
     }
 
-    function method ntt_rec3(ghost a: seq<seq<elem>>, len: pow2_t, ghost idxs: seq<seq<index_t>>): (ys: seq<seq<elem>>)
-        requires ntt_chunk_indicies_inv(a, idxs, len);
-        requires 1 <= len.full;
-        requires 0 <= len.exp <= L;
-        ensures ntt_chunks_eval_inv(a, idxs, ys, len);
-        decreases len.exp;
+    datatype level_view = level_cons(
+        ghost a: seq<seq<elem>>,
+        ghost idxs: seq<seq<index_t>>,
+        m: pow2_t)
     {
-        pow2_basics(len);
-        if len.full == 1 then 
-            ntt_rec3_base(a, len, idxs)
-        else
-            var len' := pow2_half(len);
-            var count := pow2_div(pow2(L), len).full;
-            var count' := pow2_div(pow2(L), len').full;
-            assume count' == pow2_div(pow2(L), len).full * 2;
+        predicate valid_level_view()
+        {
+            && 0 <= m.exp <= L
+            && |a| == |idxs| == chunk_count(m)
+            && (forall ki: nat | ki < |a| :: (
+                && ntt_indicies_inv(a[ki], idxs[ki], m, ki)
+                && |a[ki]| == |a[ki]| == m.full))
+        }
 
-            ghost var a' := seq(count', i  requires 0 <= i < count' => 
-                if i % 2 == 0 then even_indexed_terms(a[i/2], len)
-                else odd_indexed_terms(a[i/2], len));
+        predicate level_eval(ys: seq<seq<elem>>)
+            requires valid_level_view()
+        {
+            && |ys| == chunk_count(m)
+            && (forall ki: nat | ki < |ys| :: (
+                && |ys[ki]| == m.full
+                && poly_eval_all_points(a[ki], ys[ki], m)))
+        }
 
-            ghost var idxs' := seq(count', i  requires 0 <= i < count' => 
-                if i % 2 == 0 then even_indexed_indices(idxs[i/2], len)
-                else odd_indexed_indices(idxs[i/2], len));
-
-            assert ntt_chunk_indicies_inv(a', idxs', len') by {
-                forall i | 0 <= i < count'
-                    ensures ntt_indicies_inv(a'[i], idxs'[i], len', i);
+        function method ntt_rec3_base(): (ys: seq<seq<elem>>)
+            requires valid_level_view()
+            requires m.full == 1 && m.exp == 0;
+            ensures level_eval(ys)
+        {
+            nth_root_lemma();
+            var ys := seq(N, i requires 0 <= i < N => [Ar()[i]]);
+            assert ntt_chunks_eval_inv(a, idxs, ys, m) by {
+                forall ki: nat | ki < |a| 
+                    ensures poly_eval_all_points(a[ki], ys[ki], m)
                 {
-                    var ki := i/2;
-
-                    var ai: seq<elem> := a[i/2];
-                    var idx := idxs[i/2];
-        
-                    assert ntt_indicies_inv(a[ki], idxs[ki], len, ki);
-    
-                    if i % 2 == 0 {
-                        ghost var a_e := even_indexed_terms(ai, len);
-                        ghost var idx_e := even_indexed_indices(idx, len);
-                        even_indexed_indices_reorder(ai, idx, len, a_e, idx_e, ki);
-                    } else {
-                        ghost var a_o := odd_indexed_terms(ai, len);
-                        ghost var idx_o := odd_indexed_indices(idx, len);
-                        odd_indexed_indices_reorder(ai, idx, len, a_o, idx_o, ki);
-                    }
+                    ntt_indicies_inv_consequence0(a[ki], idxs[ki], m, ki);
+                    ntt_rec_base_case(a[ki], m);
+                    assert a[ki] == ys[ki];
                 }
             }
-            var ys' := ntt_rec3(a', len', idxs');
-
-            ntt_rec2_chunk_combine_feasible(a, a', len, count, count', idxs, idxs', ys');
-
-            var ys := seq(count, i  requires 0 <= i < count => 
-                ntt_rec2_combine(a[i], a'[2 * i], a'[2 * i + 1], len, idxs[i], ys'[i * 2], ys'[i * 2 + 1], i));
             ys
+        }
+
+        function method ntt_rec3(): (ys: seq<seq<elem>>)
+            requires valid_level_view()
+            decreases m.exp;
+        {
+            pow2_basics(m);
+            if m.full == 1 then 
+                ntt_rec3_base()
+            else
+                var m' := pow2_half(m);
+                var count := chunk_count(m);
+                var count' := chunk_count(m');
+                assume count' == count * 2;
+
+                ghost var a' := seq(count', i  requires 0 <= i < count' => 
+                    if i % 2 == 0 then even_indexed_terms(a[i/2], m)
+                    else odd_indexed_terms(a[i/2], m));
+
+                ghost var idxs' := seq(count', i  requires 0 <= i < count' => 
+                    if i % 2 == 0 then even_indexed_indices(idxs[i/2], m)
+                    else odd_indexed_indices(idxs[i/2], m));
+
+                assert ntt_chunk_indicies_inv(a', idxs', m') by {
+                    forall i | 0 <= i < count'
+                        ensures ntt_indicies_inv(a'[i], idxs'[i], m', i);
+                    {
+                        var ki := i/2;
+
+                        var ai: seq<elem> := a[i/2];
+                        var idx := idxs[i/2];
+            
+                        assert ntt_indicies_inv(a[ki], idxs[ki], m, ki);
+        
+                        if i % 2 == 0 {
+                            ghost var a_e := even_indexed_terms(ai, m);
+                            ghost var idx_e := even_indexed_indices(idx, m);
+                            even_indexed_indices_reorder(ai, idx, m, a_e, idx_e, ki);
+                        } else {
+                            ghost var a_o := odd_indexed_terms(ai, m);
+                            ghost var idx_o := odd_indexed_indices(idx, m);
+                            odd_indexed_indices_reorder(ai, idx, m, a_o, idx_o, ki);
+                        }
+                    }
+                }
+                var lv' := level_cons(a', idxs', m');
+                var ys' := lv'.ntt_rec3();
+
+                ntt_rec2_chunk_combine_feasible(a, a', m, count, count', idxs, idxs', ys');
+
+                var ys := seq(count, i  requires 0 <= i < count => 
+                    ntt_rec2_combine(a[i], a'[2 * i], a'[2 * i + 1], m, idxs[i], ys'[i * 2], ys'[i * 2 + 1], i));
+                ys
+        }        
     }
+
 }
